big step semantics

theories/Terminate.v
@@ -14,19 +14,7 @@ Open Scope nat.
 
 Create HintDb progress discriminated.
 
-Lemma hm_both_sup_p : forall {T} {P Psub} {n nsub} {ms : MergingStrategy T n}
-  {mssub : MergingStrategy T nsub} {i} {u},
-  SubStrategy Psub P i mssub ms ->
-  HieraricalMergingInv Psub mssub u ->
-  AllInUnion P u.
-Proof.
-  intros.
-  induction u.
-  - invcd H0. constructor. eapply proper_ms_sub_p; eauto.
-  - constructor; eauto with inv. 
-Qed.
-
-Theorem progress : forall {T n t} {ms : MergingStrategy T n},
+Theorem terminate' : forall {T n t} {ms : MergingStrategy T n},
   EvalTermsGood ms t ->
   (exists u, t ==>* (EvalValue ms u) /\ EvalTermsGood ms (EvalValue ms u)).
 Proof.
@@ -73,21 +61,21 @@ Proof.
     assert (exists n (s : MergingStrategy T n) ev, sub ti = Some (MSSubLt s ev))
       as [n' [s' [H5 H5']]] by eauto with strategy.
     specialize (hm_sub_st H5 H0 H5' et) as [P1 ?].
-    eapply HMSortedI; eauto with inv strategy union.
+    eapply HMSortedI; eauto 3 with inv strategy union.
   }
   (* SSEq *)
   { inversiond H4.
     specialize (hm_sub_st ev H0 H2 et) as [P1 ?].
     specialize (hm_sub_st ev H1 H2 ef) as [P2 ?].
-    assert (HieraricalMergingInv P1 s f) by eauto with inv.
+    assert (HieraricalMergingInv P1 s f) by eauto 3 with inv.
     assert (EvalTermsGood s (MrgIf s c t0 f)) by (econstructor; eauto).
     specialize (H3 _ _ H8) as [u [H8' H8'']].
     assert (SSMrgIf (SortedStrategy n ind sub0) c t0 f ==>* EvalValue (SortedStrategy n ind sub0) u)
       by (econstructor; eauto with eval).
     exists u.
     intuition.
-    invc H8''. assert (ProperStrategy P (SortedStrategy n ind sub0)) by eauto with inv.
-    assert (ProperStrategy P3 s) by eauto with inv.
+    invc H8''. assert (ProperStrategy P (SortedStrategy n ind sub0)) by eauto 3 with inv.
+    assert (ProperStrategy P3 s) by eauto 3 with inv.
     specialize (all_in_union_left_most' H0); simpl; intros.
     econstructor.
     eapply hm_sup_hm; eauto.
@@ -95,24 +83,24 @@ Proof.
   }
   (* SSGt *)
   { exists (If (pnegsb c) f t0); eauto.
-    econstructor; econstructor; eauto with eval.
-    assert (ProperStrategy P (SortedStrategy n ind sub)) by eauto with inv.
+    econstructor; econstructor; eauto 3 with eval.
+    assert (ProperStrategy P (SortedStrategy n ind sub)) by eauto 3 with inv.
     assert (exists n (s : MergingStrategy T n) ev, sub fi = Some (MSSubLt s ev))
-      as [n' [s' [H5 H5']]] by eauto with strategy.
+      as [n' [s' [H5 H5']]] by eauto 3 with strategy.
     specialize (hm_sub_st H5 H1 H5' ef) as [P1 ?].
-    eapply HMSortedI; eauto with inv strategy union.
+    eapply HMSortedI; eauto 3 with inv strategy union.
   }
   (* SIDeg *)
   { assert (EvalTermsGood (SortedStrategy n ind sub) (SSMrgIf (SortedStrategy n ind sub) c t0 f)).
-    { econstructor; eauto with eval union. }
+    { econstructor; eauto 3 with eval union. }
     specialize (H1 _ _ H3) as [u [H3' H3'']].
     exists u.
     intuition.
-    econstructor; econstructor; eauto.
+    econstructor; econstructor; eauto 2 with eval.
   }
   (* SILt *)
   { assert (EvalTermsGood (SortedStrategy n ind sub) (EvalValue (SortedStrategy n ind sub) (If c t0 (If fc ft ff)))).
-    { econstructor. eapply hm_if_no_deg; simpl; eauto with inv.
+    { econstructor. eapply hm_if_no_deg; simpl; eauto 3 with inv.
       eapply (all_in_union_left_most' H1). }
     exists (If c t0 (If fc ft ff)).
     intuition.
@@ -121,8 +109,8 @@ Proof.
     econstructor; eauto.
   }
   (* SIEq *)
-  { assert (SubUnion ft (If fc ft ff)) by eauto with union.
-    assert (ef0:HieraricalMergingInv P (SortedStrategy n ind sub) ft) by eauto with inv.
+  { assert (SubUnion ft (If fc ft ff)) by eauto 3 with union.
+    assert (ef0:HieraricalMergingInv P (SortedStrategy n ind sub) ft) by eauto 3 with inv.
     inversiond ef; repeat aiu_simplify.
     - specialize (all_in_union_left_most' H9); simpl; intro.
       rewrite H2 in H12. invc H12. lia.
@@ -130,22 +118,22 @@ Proof.
       clear ev.
       specialize (hm_sub_st ev0 H1 H20 ef0) as [P1 ?].
       specialize (hm_sub_st ev0 H0 H20 et) as [P2 ?].
-      assert (HieraricalMergingInv P1 s t0) by eauto with inv.
+      assert (HieraricalMergingInv P1 s t0) by eauto 3 with inv.
       clear P2 H12.
       assert (EvalTermsGood s (MrgIf s c t0 ft)).
-      { econstructor; eauto with eval. }
+      { econstructor; eauto 3 with eval. }
       specialize (H5 _ _ H12) as [u [H5' H5'']].
       exists (If (porsb c fc) u ff).
       intuition.
       econstructor.
-      eapply SIEq; eauto.
+      eapply SIEq; eauto 3 with eval.
       constructor.
 
       assert (SubStrategy P1 P z s (SortedStrategy n ind sub)).
       { specialize (all_in_union_left_most' H0); simpl; intros.
         econstructor; eauto with inv. }
       invcd H5''.
-      assert (HieraricalMergingInv P1 s u) by eauto with inv.
+      assert (HieraricalMergingInv P1 s u) by eauto 3 with inv.
       clear P0 H19.
 
       econstructor.
@@ -155,71 +143,71 @@ Proof.
       auto.
   }
   (* SIGt *)
-  { assert (SubUnion ft (If fc ft ff)) by eauto with union.
+  { assert (SubUnion ft (If fc ft ff)) by eauto 3 with union.
     inversiond ef; repeat aiu_simplify.
     - specialize (all_in_union_left_most' H9); simpl; intro.
       rewrite H2 in H12. invc H12. lia.
     - assert (EvalTermsGood (SortedStrategy n ind sub) (MrgIf (SortedStrategy n ind sub) c t0 ff)).
-      { econstructor; eauto with inv. }
+      { econstructor; eauto 3 with inv. }
       specialize (H5 _ _ H12) as [u [H5 H5']].
       exists (If (pandsb (pnegsb c) fc) ft u).
       intuition.
-      { econstructor. eapply SIGt; eauto.
+      { econstructor. eapply SIGt; eauto 3 with eval.
         constructor. 
       }
       invcd H5'.
-      assert (HieraricalMergingInv P (SortedStrategy n ind sub) u) by eauto with inv.
+      assert (HieraricalMergingInv P (SortedStrategy n ind sub) u) by eauto 3 with inv.
       clear P0 H18.
       
       econstructor.
-      eapply HMSortedI; repeat aiu_simplify; eauto with inv; try solve_aiu.
-      eapply eval_do_not_change_index_lowerbound; eauto.
+      eapply HMSortedI; repeat aiu_simplify; eauto 3 with inv; try solve_aiu.
+      eapply eval_do_not_change_index_lowerbound; eauto 3 with eval.
 
       constructor; solve_aiu.
   }
   (* ISDeg *)
   { assert (EvalTermsGood (SortedStrategy n ind sub) (SSMrgIf (SortedStrategy n ind sub) c t0 f)).
-    { econstructor; eauto with eval union. }
+    { econstructor; eauto 3 with eval union. }
     specialize (H1 _ _ H3) as [u [H3' H3'']].
     exists u.
     intuition.
-    econstructor; econstructor; eauto.
+    econstructor; econstructor; eauto 2 with eval.
   }
   (* ISLt *)
   { assert (EvalTermsGood (SortedStrategy n ind sub) (MrgIf (SortedStrategy n ind sub) c tf f)).
-    { econstructor; eauto with eval union inv. }
+    { econstructor; eauto 2 with eval union inv. }
     specialize (H5 _ _ H7) as [f' [H5 H5']].
     invcd H5'.
-    assert (ProperStrategy P (SortedStrategy n ind sub)) by eauto with inv.
+    assert (ProperStrategy P (SortedStrategy n ind sub)) by eauto 2 with inv.
     specialize (all_in_union_left_most' H0); simpl; intros.
     specialize (proper_ms_ind_some_is_sub_some H8 H9) as [n' [ev' [s' ?]]].
     specialize (proper_ms_sub_from_subfunc H8 H9 H12) as [Psub ?].
-    assert (HieraricalMergingInv P (SortedStrategy n ind sub) tt) by eauto with inv.
-    assert (HieraricalMergingInv Psub s' tt) by eauto with subinv.
+    assert (HieraricalMergingInv P (SortedStrategy n ind sub) tt) by eauto 2 with inv.
+    assert (HieraricalMergingInv Psub s' tt) by eauto 2 with subinv.
     exists (If (pandsb c tc) tt f').
     intuition.
-    - econstructor. eapply ISLt; eauto. econstructor.
+    - econstructor. eapply ISLt; eauto 2 with eval. econstructor.
     - econstructor. eapply HMSortedI. 4: apply H12.
       all: repeat aiu_simplify; eauto. all: eauto 4 with inv.
-      eapply eval_do_not_change_index_lowerbound; eauto.
+      eapply eval_do_not_change_index_lowerbound; eauto 2 with eval.
       simpl. intuition; eauto 3 with union.
       invcd et; try solve_aiu.
       repeat aiu_simplify. assert (z = tfi) by eauto with union. lia.
   }
   (* ISEq *)
-  { assert (ProperStrategy P (SortedStrategy n ind sub)) by eauto with inv.
+  { assert (ProperStrategy P (SortedStrategy n ind sub)) by eauto 2 with inv.
     specialize (all_in_union_left_most' H1); simpl; intros.
     specialize (proper_ms_sub_from_subfunc H7 H8 H4) as [Psub ?].
-    assert (HieraricalMergingInv P (SortedStrategy n ind sub) tt) by eauto with inv.
-    assert (HieraricalMergingInv Psub s tt) by eauto with subinv.
+    assert (HieraricalMergingInv P (SortedStrategy n ind sub) tt) by eauto 2 with inv.
+    assert (HieraricalMergingInv Psub s tt) by eauto 2 with subinv.
     assert (EvalTermsGood s (MrgIf s c tt f)).
-    { econstructor; eauto with subinv. }
+    { econstructor; eauto 2 with subinv. }
     specialize (H5 _ _ H13) as [t' [H5 H5']].
     invcd H5'.
-    assert (HieraricalMergingInv Psub s t') by eauto with inv.
+    assert (HieraricalMergingInv Psub s t') by eauto 3 with inv.
     exists (If (porsb (pnegsb c) tc) t' tf).
     intuition.
-    - econstructor. eapply ISEq; eauto. econstructor.
+    - econstructor. eapply ISEq; eauto 2 with eval. econstructor.
     - econstructor. eapply HMSortedI. 4: apply H4.
       all: repeat aiu_simplify; eauto. all: eauto 3 with inv.
       + eapply hm_both_sup_p; eauto.
@@ -242,74 +230,74 @@ Proof.
   }
 
   (* IIDeg1 *)
-  { assert (AllInUnion (fun x => AllInUnion (fun y => ind x = ind y) t0) t0) by eauto with union.
+  { assert (AllInUnion (fun x => AllInUnion (fun y => ind x = ind y) t0) t0) by eauto 2 with union.
     assert (EvalTermsGood (SortedStrategy n ind sub) (SIMrgIf (SortedStrategy n ind sub) c t0 f)).
-    { eauto with eval. }
+    { eauto 2 with eval. }
     specialize (H1 _ _ H4) as [u [H1 H1']].
     exists u.
     intuition.
-    econstructor. eapply IIDeg1; eauto. constructor.
+    econstructor. eapply IIDeg1; eauto 2 with eval. constructor.
   }
 
   (* IIDeg2 *)
-  { assert (AllInUnion (fun x => AllInUnion (fun y => ind x = ind y) f) f) by eauto with union.
+  { assert (AllInUnion (fun x => AllInUnion (fun y => ind x = ind y) f) f) by eauto 2 with union.
     assert (EvalTermsGood (SortedStrategy n ind sub) (ISMrgIf (SortedStrategy n ind sub) c (If tc tt tf) f)).
-    { eauto with eval. }
+    { eauto 2 with eval. }
     specialize (H4 _ _ H7) as [u [H4 H4']].
     exists u.
     intuition.
-    econstructor. eapply IIDeg2; eauto. constructor.
+    econstructor. eapply IIDeg2; eauto 2 with eval. constructor.
   }
 
   (* IILt *)
   { assert (EvalTermsGood (SortedStrategy n ind sub)
                           (MrgIf (SortedStrategy n ind sub) c tf (If fc ft ff))).
-    { econstructor; eauto with eval union inv. }
+    { econstructor; eauto 2 with eval union inv. }
     specialize (H7 _ _ H9) as [f' [H7 H7']].
     exists (If (pandsb c tc) tt f').
 
     intuition.
-    econstructor. eapply IILt; eauto. constructor.
+    econstructor. eapply IILt; eauto 2 with eval. constructor.
 
-    assert (ProperStrategy P (SortedStrategy n ind sub)) by eauto with inv.
+    assert (ProperStrategy P (SortedStrategy n ind sub)) by eauto 2 with inv.
     specialize (all_in_union_left_most' H0); simpl; intros.
     specialize (proper_ms_ind_some_is_sub_some H10 H11) as [n' [ev' [s' ?]]].
     specialize (proper_ms_sub_from_subfunc H10 H11 H12) as [Psub ?].
-    assert (HieraricalMergingInv P (SortedStrategy n ind sub) tt) by eauto 3 with inv.
-    assert (HieraricalMergingInv Psub s' tt) by eauto with subinv.
+    assert (HieraricalMergingInv P (SortedStrategy n ind sub) tt) by eauto 2 with inv.
+    assert (HieraricalMergingInv Psub s' tt) by eauto 2 with subinv.
     invcd H7'.
     assert (HieraricalMergingInv P (SortedStrategy n ind sub) f') by eauto 3 with inv.
 
     econstructor. eapply HMSortedI; eauto; repeat aiu_simplify; eauto 3 with inv.
-    eapply eval_do_not_change_index_lowerbound; eauto.
-    simpl. intuition; eauto 3 with union.
-    invcd et; try solve_aiu.
-    repeat aiu_simplify. assert (z = tfi) by eauto with union. lia.
+    eapply eval_do_not_change_index_lowerbound; eauto 2 with eval.
+    simpl. intuition; eauto 2 with union.
+    { invcd et; try solve_aiu.
+      repeat aiu_simplify. assert (z = tfi) by eauto with union. lia. }
 
-    eapply hm_lm_is_lowerbound; eauto.
-    simpl. exact (all_in_union_left_most' H2).
+    { eapply hm_lm_is_lowerbound; eauto.
+      simpl. exact (all_in_union_left_most' H2). }
   }
 
   (* IIEq *)
   { assert (EvalTermsGood (SortedStrategy n ind sub)
                           (MrgIf (SortedStrategy n ind sub) c tf ff)).
-    { econstructor; eauto with eval union inv. }
+    { econstructor; eauto 2 with eval union inv. }
     specialize (H8 _ _ H10) as [f' [H8 H8']].
 
-    assert (ProperStrategy P (SortedStrategy n ind sub)) by eauto with inv.
+    assert (ProperStrategy P (SortedStrategy n ind sub)) by eauto 2 with inv.
     specialize (all_in_union_left_most' H0); simpl; intros.
     specialize (proper_ms_sub_from_subfunc H11 H12 H6) as [Psub ?].
     assert (HieraricalMergingInv P (SortedStrategy n ind sub) tt) by eauto 2 with inv.
-    assert (HieraricalMergingInv Psub s tt) by eauto with subinv.
+    assert (HieraricalMergingInv Psub s tt) by eauto 2 with subinv.
     assert (HieraricalMergingInv P (SortedStrategy n ind sub) ft) by eauto 2 with inv.
-    assert (HieraricalMergingInv Psub s ft) by eauto with subinv.
+    assert (HieraricalMergingInv Psub s ft) by eauto 2 with subinv.
     assert (EvalTermsGood s (MrgIf s c tt ft)).
-    { econstructor; eauto with subinv. }
+    { econstructor; eauto 2 with subinv. }
     specialize (H7 _ _ H21) as [t' [H7 H7']].
     exists (If (pitesb c tc fc) t' f').
 
     intuition.
-    econstructor. eapply IIEq; eauto. constructor.
+    econstructor. eapply IIEq; eauto 2 with eval. constructor.
 
     invcd H8'.
     assert (HieraricalMergingInv P (SortedStrategy n ind sub) f') by eauto 3 with inv.
@@ -320,8 +308,8 @@ Proof.
 
     - eapply hm_both_sup_p; eauto.
     - eapply eval_do_not_change_index_sub_eq; simpl; eauto; intuition; eauto.
-    - eapply eval_do_not_change_index_lowerbound; eauto.
-      simpl. intuition; eauto 3 with union.
+    - eapply eval_do_not_change_index_lowerbound; eauto 2 with eval.
+      simpl. intuition; eauto 2 with union.
       + invcd et; try solve_aiu.
         repeat aiu_simplify. assert (z = tfi) by eauto 4 with union. lia.
       + invcd ef; try solve_aiu.
@@ -331,25 +319,25 @@ Proof.
   (* IIGt *)
   { assert (EvalTermsGood (SortedStrategy n ind sub)
                           (MrgIf (SortedStrategy n ind sub) c (If tc tt tf) ff)).
-    { econstructor; eauto with eval union inv. }
+    { econstructor; eauto 2 with eval union inv. }
     specialize (H7 _ _ H9) as [f' [H7 H7']].
     exists (If (pandsb (pnegsb c) fc) ft f').
 
-    assert (ProperStrategy P (SortedStrategy n ind sub)) by eauto with inv.
+    assert (ProperStrategy P (SortedStrategy n ind sub)) by eauto 2 with inv.
     specialize (all_in_union_left_most' H2); simpl; intros.
     specialize (proper_ms_ind_some_is_sub_some H10 H11) as [n' [ev' [s' ?]]].
     specialize (proper_ms_sub_from_subfunc H10 H11 H12) as [Psub ?].
-    assert (HieraricalMergingInv P (SortedStrategy n ind sub) ft) by eauto 3 with inv.
-    assert (HieraricalMergingInv Psub s' ft) by eauto with subinv.
+    assert (HieraricalMergingInv P (SortedStrategy n ind sub) ft) by eauto 2 with inv.
+    assert (HieraricalMergingInv Psub s' ft) by eauto 2 with subinv.
     invcd H7'.
     assert (HieraricalMergingInv P (SortedStrategy n ind sub) f') by eauto 3 with inv.
 
     intuition.
-    econstructor. eapply IIGt; eauto. constructor.
+    econstructor. eapply IIGt; eauto 2 with eval. constructor.
 
     econstructor. eapply HMSortedI; eauto; repeat aiu_simplify; eauto 3 with inv.
-    eapply eval_do_not_change_index_lowerbound; eauto.
-    simpl. intuition; eauto 3 with union.
+    eapply eval_do_not_change_index_lowerbound; eauto 2 with eval.
+    simpl. intuition; eauto 2 with union.
 
     - assert (fti < tti)%Z by lia. eapply hm_lm_is_lowerbound; eauto.
       simpl. exact (all_in_union_left_most' H0). 
@@ -359,7 +347,23 @@ Proof.
   }
 Qed.
 
+Definition is_value {T} (v : EvalTerms T) : Prop :=
+  match v with
+  | EvalValue _ _ => True
+  | _ => False
+  end.
 
-  
-  
+Theorem terminate : forall {T n t} {ms : MergingStrategy T n},
+  EvalTermsGood ms t ->
+  ~is_value t ->
+  (exists u, t ==> (EvalValue ms u) /\ EvalTermsGood ms (EvalValue ms u)).
+Proof.
+  intros.
+  specialize (terminate' H) as [u [? ?]].
+  specialize (eval_star_is_eq_or_onestep H1).
+  intuition; subst.
+  - exfalso; simpl in *; auto. 
+  - exists u.
+    destruct t; intuition.
+Qed.
   
